## Aufgabe 1
$f'(x) = 2x +4$
$f'(-1) = 2$

$$m = \frac{\Delta y}{\Delta x} = \frac{y_2 - y_1}{x_2 - x_1}$$
$f(-0.9) = 0.81 -3.6 +4 = 1.21$
$m_{P_0,P_2} = \frac{21}{10}$

## Aufgabe 2
### a)
$f(x) = 3x^3 -3x^2 -12x +12$
$f'(x) = 9x^2 -6x -12$
$m_{\frac12} = f'(\frac12) = -\frac{51}4$
$y_{\frac12} = f(\frac12) = \frac38 -\frac34 -6 +12 = \frac{45}{8}$
$\frac{45}8 = -\frac{51}4*\frac12 +n$ $|$
$\frac{45}8 = -\frac{51}8 +n$ $|+\frac{51}8$
$n_{\frac12} = \frac{96}8 = 12$
$t_{\frac12}: y = -\frac{51}4x +12$

## Aufgabe 3
$f(x) = \frac23x^3 -2x^2 -1$
$f'(x) = 2x^2 -4x$
### a)
$0 = 2x^2 -4x$ $|:2$
$0 = x^2 -2x$
$x_{1,2} = 1 \pm 1$
$x_1 = 0$
$x_2 = 2$

$P_1(0|-1)$
$P_2(2|-\frac{11}3)$

### b)
$-2 = 2x^2 -4x$ $|+2$
$0 = 2x^2 -4x +2$ $|:2$
$0 = x^2 -2x +1$
$x = 1$

$P(1|-\frac73)$

### c)
$6 = 2x^2 -4x$ $|-6$
$0 = 2x^2 -4x -6$ $|:2$
$0 = x^2 -2x -3$
$x_{1,2} = 1 \pm 2$
$x_1 = -1$
$x_2 = 3$

$P(-1|-\frac{11}3)$
$P(3|-1)$

## Aufgabe 4
### a)
$f(x) = 3x^2$
$f'(x) = 6x$

$g(x) = 2x^3$
$g'(x) = 6x^2$

$f'(x) = g'(x)$
$6x = 6x^2$ $|:6$
$x = x^2 \implies x_1 = 0, x_2 = 1$

### b)
$f(x) = x^3 +\frac52x^2 -18x +2$
$f'(x) = 3x^2 +5x -18$

$g(x) = -2x^2 +12x -64$
$g'(x) = -4x +12$

$f'(x) = g'(x)$
$3x^2 +5x -18 = -4x +12$ $|+4x, -12$
$0 = 3x^2 +9x -30$ $|:3$
$0 = x^2 +3x -10$
$x_{1,2} = -1.5 \pm \frac72$
$x_1 = -5$
$x_2 = 2$

## Aufgabe 5
$f(x) = 2x^3 +4x^2 -8x +1$
$f'(x) = 6x^2 +8x -8$

$m_{\frac12} = -2.5$
$y_{\frac12} = -1.75$
$-1.75 = -1.25 +n_{\frac12}$ $|+1.75$
$0 = 0.5 +n_{\frac12} \implies n_{\frac12} = -0.5$
$t_{\frac12}: y = -2.5x -0.5$

$m_1 = 6$
$y_1 = -1$
$-1 = 6 +n \implies n = -7$
$t_1: y = 6x -7$

$-\frac52x -\frac12 = 6x -7$ $|+\frac52x; +7$
$\frac{13}2 = \frac{17}2x$ $|*\frac2{17}$
$\frac{13}{17} = x$

$\arctan{|\frac{m_2 - m_1}{1 + m_1 * m_2}|}$
$\varphi = arctan{|\frac{6+2.5}{1-2.5*6}|}$
$\varphi = arctan{|-\frac{8.5}{14}|}$
$\varphi = arctan{\frac{17}{28}}$
