## Nr.1
### a)
$f(x) = \frac5{12}x^6 -\frac37x^5 +\frac73x^4 -\frac23x -2$

### c)
$f(x) = 5x^{\frac13} -5x^{-1}$
$f'(x) = \frac53x^{-\frac23} +5x^{-2}$

### d)
$f(x) = \frac43e^x -\frac23\sin x$

## Nr.2
$f(x) = \frac5{18}x^3 -\frac14x^2 -\frac23x$
$f'(x) = \frac56x^2 -\frac12x -\frac23$
$f'(-3) = \frac56*9 +\frac32 -\frac23 = \frac{45 +9 -4}{6} = \frac{25}3 = m$
$f(-3) = \frac{-30 -9 +8}{4} = -\frac{31}4 = y$
$-\frac{31}4 = \frac{25}4 *(-3) +n$
$n = -\frac{31}4 +25 = \frac{69}4$
$t: y = \frac{25}3x +\frac{69}4$

## Nr.3
$f(x) = \frac12x^3 +3x^2 +4x$
$g: y = \frac43x + \frac53$
$f'(x) = \frac32x^2 +6x +4$
$-\frac43 = \frac32x^2 +6x +4$ $|+\frac43$
$0 = \frac32x^2 +6x +\frac{16}3$ $|*\frac23$
$0 = x^2 +4x +\frac{32}9$
$x_{1,2} = -2 \pm \sqrt{4 -\frac{32}9} = -2 \pm \frac23$
$x_1 = -\frac43$
$x_2 = -\frac83$

## Nr.4
$f(x) = \frac43x -\frac{14}3\sin x$
$f'(x) = \frac43 -\frac{14}3\cos x$
$f'(\pi) = 6$
$m_n = -\frac16$
$f(\pi) = \frac43\pi$
$\frac43\pi = -\frac16\pi +n$
$n = \frac43\pi +\frac16\pi = \frac{3}{2}\pi$
Normale: $y = -\frac16x +\frac32\pi \implies S_y(0|\frac32)\pi$
$0 = -\frac16x +\frac32\pi$ $|+\frac16x$
$\frac16x = \frac32\pi$
$x = 9\pi \implies S_x(9\pi|0)$
