.# Nr.2
## a)
$A(2|0)$ $B(-2|4)$ $C(-4|8)$ $H(0|f(0)))$

$f(2) = 0$
$f(-2) = 4$
$f(-4) = 8$
$f'(0) = 0$

???

## b)
$B(0 |0)$ $P(-3|0)$ $m_{P} = 6$

$f(0) = 0$
$f'(0) = 0$
$f(-3|0)$
$f'(-3) = 6$

$f(x) = \frac{2}{3}x^3 +2x^2$

## c)
$E(1|4)$ $W(0|2)$

$f(1) = 4$
$f'(1) = 0$
$f(0) = 2$
$f''(0) = 0$

$f(x) = -x^3 +3x +2$

# Nr.3
form: $ax^4 +bx^3 +cx^2 +dx +e$

## a)
form: $ax^4 +bx^2 +c$
$f(0) = 2$
$f(1) = 0$
$f'(1) = 0$

$f'(x) = 4ax^3 +2bx$

  I. $f(0) = c = 2$
 II. $f(1) = a +b +c = 0$
III. $f'(1) = 4a +2b = 0$

$b = -2a$
$-a +c = 0$

$a = -2$
$b = 4$
$c = 2$

## b)
form: $ax^4 +bx^2 +c$
$f(2) = 0$
$f'(2) = -\frac{4}{3}$
$f''(2) = 0$

$f'(x) = 4ax^3 +2bx$
$f''(x) = 12ax^2 +2b$

  I. $f(2) = 16a +4b +c = 0$
 II. $f'(2) = 32a +8b = -\frac{4}{3}$
III. $f''(2) = 48a +2b = 0$

$b = -24a$
$c = -(16a -96a)$
$c = 80a$

$32a +8b = -\frac{4}{3}$
$-160a = -\frac{4}{3}$
$a = -\frac{4}{3} \cdot -\frac{1}{160}$
$a = -\frac{1}{3} \cdot -\frac{1}{40}$
$a = \frac{1}{120}$
$b = -24\cdot \frac{1}{120} = -\frac{1}{5}$
$c = 80 \cdot \frac{1}{120} = \frac{2}{3}$

# Nr. 4
form: $f(x) = a(x+b)e^{kx}$ 
## a)
$f(0) = -2$
$f'(1) = 0$
$f(0) = 5$

$f(x) = \frac{5}{2}\cdot(x+2)\cdot e^{-\frac{1}{3}x}$

## b)
$f(3) = 0$
$f''(2) = 0$
$f'(2) = -\frac{1}{10}e^4$

$f(x) = \frac{1}{10}\cdot(x-3)\cdot e^{2x}$
$f(x) = -\frac{1}{10}\cdot(x-3)\cdot e^4 \implies$ lineare Funktion, entf√§llt

# Nr.5
form: $f(x) = a\cdot \sin(\pi x+c)+d$
## a)
  I. $f(0) = 4$
 II. $f(2) = 4$
III. $f'(2) = 3\pi$
 IV. $c = 0$

$f(x) = 3\cdot\sin(\pi\cdot x)+4$

## b)
  I. $f\left( \frac{3}{4} \right) = -\frac{3}{4}$
 II. $f'\left( \frac{3}{4} \right) = 0$
III. $f''\left( \frac{1}{4} \right) = 0$
 IV. $f'\left( \frac{1}{4} \right) = \frac{\pi}{4}$

$f(x) = -\frac{1}{4}\sin\left( x\cdot \pi+\frac{3}{4}\pi \right)-1$

# Nr.6
## a)
$f(x) = ax^4+bx^3+cx^2+dx+e$
$f(x) = ax^4+bx^2+c$

  I. $f(-2) = 5$
 II. $f'(-2) = 0$
III. $f(0) = -3$
 IV. $f'(0) = 0$
  V. $f(2) = 5$

$f(x) = -\frac{1}{2}x^4+4x^2-3$

## b)
$f(x) = a\cdot \sin\left( \frac{\pi}{2}x +c \right) +d$

  I. $f(0.5) = 0$
 II. $f(1.5) = 1.5$
III. $f'(1.5) = 0$
 
$f(x) = -\frac{3}{2}\cdot \sin\left( \frac{\pi}{2}x+\frac{3}{4}\pi \right)$

## c)
$f(x) = a(x+b)e^{kx}$

  I. $f'(-1) = 0$
 II. $f(0) = -2$
III. $f(1) = 0$

$f(x) = 2\cdot(x-1)\cdot e^{\frac{1}{2}x}$
