# Nr. 1
- 2 A
- 3 A
- 4 A
- 5 B!
- 6 A
- 7 A
- 8 A
- 9 A
- 10 A
- 11 A
- 12 B!
- 13 B!

# Nr. 2
$f(x) = ax^3 +bx^2 +cx$
$f'(x) = 3ax^2 +2bx +c$

  I. $f'(0) = c = 0$
 II. $f(-3) = -27a +9b -3c = 0$
III. $f'(-3) = 27a -6b + c = 9$

$3b - 2c= 9$ <- II. + III.
$3b -2\cdot0 = 9 \implies b = 3$
$27a -18 +0 = 9 \implies a = 1$

# Nr. 3
$f(x) = ax^3 +bx^2 +cx$
$f'(x) = 3ax^2 +2bx +c$
$f''(x) = 6ax +2b$

  I. $f'(2) = 12a +4b +c = 0$
 II. $f''(4) = 24a +2b = 0 \implies b = -12a$
III. $f'(4) = 48a + 8b +c = -4$

$-36a +c = 0 \implies c = 36a$
$48a -96a +36a = -12a = -4 \implies a = \frac{1}{3}$
$b = -12a = -4$
$c = 36a = 12$

# Nr. 4
$f(x) = ax^4 +bx^2 +c$
$f'(x) = 4ax^3 +2bx$
$f''(x) = 12ax^2 + 2b$

  I. $f(2) = 16a + 4b +c = 0$
 II. $f'(2) = 32a +4b = 2$
III. $f''(-1) = 12a +2b = 0 \implies b = -6a$

$32a - 24a = 2 \implies a = \frac{1}{4}$
$b = -\frac{3}{2}$
$16a -24a +c = 0 \implies c = 8a$
$c = 2$


# Nr. 7
form:
$ax^5 +bx^3 +cx$
