$f(x) = ax^3 +bx^2 +cx +d$
# a)

   I. $f''(5) = 0$

$f(x)_{a;c;d} = ax^3 -15ax^2 +cx +d$ $a\neq0$

# b)

   I. $f''(5) = 0$
  II. $f'(1) = 0$

$f(x)_{a;d} = ax^3 -15ax^2 +27ax +d$ $a\neq0$

# c)

   I. $f''(3) = 0$
  II. $f'(0) = 0$
 III. $f'(6) = 0$

$f(x)_{a;d} = ax^3 -9ax^2 +d$ $a\neq0$

# d)

   I. $f''(3) = 0$
  II. $f'(3) = 1$
 III. $f'(0) = 0$
  IV. $f'(6) = 0$

$f(x)_{d} = -\frac{1}{27}x^3 +\frac{1}{3}x^2 +d$

# e)

   I. $f''(3) = 0$
  II. $f'(3) = 1$
 III. $f'(0) = 0$
  IV. $f'(6) = 0$
   V. $f(0) = 5$

$f(x) = -\frac{1}{27}x^3 +\frac{1}{3}x^2 +5$
# f)

   I. $f''(3) = 0$
  II. $f'(3) = 1$
 III. $f'(0) = 0$
  IV. $f'(6) = 0$
   V. $f(0) = 5$
  VI. $f(1) = 0$

Keine LÃ¶sung
