# 1
$\vec{a} = \begin{pmatrix} 7 \\ 1 \\ -2 \end{pmatrix}$
$\vec{b} = \begin{pmatrix} 0 \\ 1 \\ -9 \end{pmatrix}$ 
$\vec{c} = \begin{pmatrix} -1 \\ 2 \\ -7 \end{pmatrix}$
$\vec{d} = \begin{pmatrix} -2 \\ 16 \\ 10 \end{pmatrix}$

# 2
$\vec{a} = \begin{pmatrix} 1 \\ -1 \\ -2 \end{pmatrix}+\begin{pmatrix} 6 \\ -3 \\ 3 \end{pmatrix} = \begin{pmatrix} 7 \\ -4 \\ 1 \end{pmatrix}$
$\vec{b} = 2 \cdot\begin{pmatrix} 2 \\ 5 \\ -1 \end{pmatrix} + \begin{pmatrix} -5 \\ 7 \\ -2 \end{pmatrix} = \begin{pmatrix} -1 \\ 17 \\ -4 \end{pmatrix}$
$\vec{c} = \begin{pmatrix} 1 \\ -1 \\ -2 \end{pmatrix} -\begin{pmatrix} -5 \\ 7 \\ -2 \end{pmatrix} - \frac{1}{2}\cdot\begin{pmatrix} 4 \\ -8 \\ 4 \end{pmatrix} = \begin{pmatrix} 4 \\ -4 \\ -2 \end{pmatrix}$

# 3
## a
$\begin{pmatrix} 2 \\ 4 \\ -3 \end{pmatrix} = \begin{pmatrix} 4 \\ 8 \\ -6 \end{pmatrix}$
$\begin{pmatrix} -7 \\ -5 \\ 5 \end{pmatrix} = \begin{pmatrix} -5 \\ -1 \\ 2 \end{pmatrix}$

--> **kein** Parallelogramm

## b
$\begin{pmatrix} 7 \\ 3 \\ 2 \end{pmatrix} = \begin{pmatrix} 7 \\ 3 \\ 2 \end{pmatrix}$

--> ein Parallelogramm

## c
$\begin{pmatrix} -3 \\ 3 \\ 5 \end{pmatrix} = \begin{pmatrix} 3 \\ -3 \\ 5 \end{pmatrix}$
$\begin{pmatrix} -5 \\ 5 \\ 6 \end{pmatrix} = \begin{pmatrix} 1 \\ -1 \\ -4 \end{pmatrix}$

--> **kein** Parallelogramm

# 4
$\vec{BC}=\begin{pmatrix} 1 \\ -1 \\ 0 \end{pmatrix}$

($A + \vec{BC} = D$) // we don't like this
$D(3|3|1)$

# 5
