# Aufgabe A1
$f(x) = x^3 +ax^2 -\frac34a^2x$
$0 = x^3 +ax^2 -\frac34a^2x$
$0 = x(x^2 +ax -\frac34a^2)$
$x_1 = 0$

$0 = x^2 +ax -\frac34a^2$
$x_{2;3} = -\frac12a \pm \sqrt{\frac14a^2 +\frac34a^2}$
$x_{2;3} = -\frac12a \pm |a|$
$x_2 = -\frac12a - |a|$
$x_3 = -\frac12a +|a|$

Für $a \geq 0$:
- $x_2 = -\frac12a -a = -\frac32a$
- $x_3 = -\frac12a +a = \frac{1}2a$

Für $a < 0$
- $x_2 = \frac12a -(-a) = \frac32a$
- $x_3 = \frac12a -a = -\frac12a$

Für $a = 0$: Nur $x_1 = 0$, also eine Lösung.
Für $a \neq 0$: $x_1 = 0$, $x_2 = \frac{3a}2$ and $x_3 = -\frac a2$, also 3 Lösungen

# Aufgabe A2
$f_a(x) = \frac1ax^2 -2x +6 = 1a^{-1} x^2 -2x +6$
$P_a(4|f_a(4))$
$S(-1|0)$

$f_a'(x) = a^{-1}2x -2$

$f_a'(4) = \frac8a -2$
$f_a(4) = \frac{16}a -2$

$\frac{16}a -2 = \frac{32}a -8 +n$
$n = -\frac{16}a +6$

$t: y = (\frac8a -2)x -\frac{16}a +6$

$0 = -\frac8a +2 -\frac{16}a +6$ $|$
$0 = -\frac{24}a +8$ $|+\frac{24}a$
$\frac{24}a = 8$ $|\cdot a$; $:8$
$a = \frac{24}8 = 3$

# Aufgabe A3
$f_a(x) = 3e^{ax} +2x$
$m = -4$

$f_a(0) = 3$
$P(0|3)$

$f_a'(x) = 3ae^{ax} +2$
$f_a'(0) = 3a +2$

$-4 = 3a +2$
$\underline{\underline{a = -2}}$

$3 = (3a +2) \cdot 0 +n$
$n = 3$

$\underline{\underline{t: y = -4x +3}}$

# Aufgabe A4
$f_a(x) = ae^{a+x}$ ($x \in R$)
Tangente $t_a$ im Punkt $P(-1|f_a(-1))$

## 4.1
$y = a \cdot e^{a-1} \cdot x +2ae^{a-1}$

$f_a(-1) = a\cdot e^{a-1}$

$f_a'(x) = ae^{a+x}$
$f_a'(-1) = a\cdot e^{a-1}$

$a \cdot e^{a-1} = -a\cdot e^{a-1} +n$
$n = 2ae^{a-1}$

$t_a: y = ae^{a-1} \cdot x +2ae^{a-1}$
$\underline{\underline{ t_a(x) = ae^{a-1}x +2ae^{a-1} }}$

## 4.2
$t_a(0) = 2ae^{a-1}$
$S_y(0|2ae^{a-1})$

$0 = t_a(x) = ae^{a-1} \cdot x +2ae^{a-1}$
$ae^{a-1}x = -2ae^{a-1}$
$x = -2$
$S_x(-2|0)$

$\frac12 \cdot |-2| \cdot |2ae^{a-1}| = 2ae^{a-1}$
$\underline{\underline{ A = 2ae^{a-1}FE }}$

# Aufgabe B1
