# Nr.2
## a)
I.   $3x -y -z = 2$
II.  $x +2y +2z = 10$
III. $-2x +5y -z = -14$

IV.  $9y +3z = 6$ <- 2II. +III.
V.   $-7y -7z = -28$ <- I. -3II.
VI.  $42y = -42$ <- 3V. +7IV.

$y = -1$
$-9 +3z = 6$
$z = 5$

$3x -4 = 2$
$x = 2$

## b)
I.   $x +2y -z = 7$
II.  $2x -y +z = 4$
III. $-x +8y -5z = 3$

IV.  $10y -6z = 10$ <- I. +III.
V.   $15y -9z = 10$ <- II. +2III.
VI.  $0 \neq 10$ <- 3IV. -2V.
$\implies$ not solution

## c)
I.   $3x -2y +5z = 13$
II.  $-x +3y +4z = -1$
III. $5x +6y -z = 3$

IV.  $7y +17z = 10$ <- I. +3II.
V.   $21y +19z = -2$ <- III. +5II.
VI.  $32z = 32$ <- 3IV. -V.
$z = 1$

$7y +17 = 10$
$y = -1$

$3x +2 +5 = 13$
$x = 2$

## d)
I.   $-2x +y -z = 5$
II.  $x +y +z = 1$
III. $2x -y +z = -5$

IV.  $3y +z = 7$ <- I. +2II.
V.   $-3y -z = -7$ <- III. -2II.
VI.  $0 = 0$ <- I. +II.
VII. $3y +z = 7$ <- 2II. -III.

VIII.$-x +2y = 6$ <- II. +I.
IX.  $x -2y = 6$ <- III. -II.

X.   $-3x -2z = 4$ <- I. -II.
XI.  $3x +2z = -4$ <- II. +III.

XII. $6y +2z = 14$ <- 3VIII. -X.
$6y = 14 -2z$
$3y = 7 -z$
$y = -\frac 13z +\frac73$

$-2x +\frac73 -\frac z3 -z = 5$
$-2x -\frac z3 -z = \frac83$
$-\frac z3 -z -\frac83= 2x$
$x = -\frac z6 -\frac z2 -\frac43 = -\frac{2}{3}z-\frac{4}{3}$

$z \in \mathbb{R}$
