$f_{t}(x) = \frac{tx-2}{x^2} = (tx -2)x^{-2} = tx^{-1} -2x^{-2}$

# a)
$f_{t}'(x) = -tx^{-2} +4x^{-3}$
$0 = -tx^{-2} +4x^{-3}$
$-tx^{-2} = -4x^{-3}$ $|\cdot x^{3}$
$-tx = -4$
$x = \frac{4}{t}$

$f_{t}''(x) = 2tx^{-3} -12x^{-4}$

$f_{t}\left( \frac{4}{t} \right) = t\left( \frac{4}{t} \right)^{-1} -2\left( \frac{4}{t} \right)^{-2})$
$f_{t}\left( \frac{4}{t} \right) = t\left( \frac{t}{4} \right) -2\left( \frac{t}{16} \right)$
$f_{t}\left( \frac{4}{t} \right) = \frac{t^{2}}{4}  -\frac{t^{2}}{8}$
$f_{t}\left( \frac{4}{t} \right) = \frac{t^2}{8}$

$t = \frac{4}{x}$
$y = \frac{\left( \frac{4}{x} \right)^2}{8} = \frac{16}{8x^2} = \frac{2}{x^2}$
$E(x) = \frac{2}{x^2}$
# b)
$f_{t}''(x) = 0$
$2tx^{-3} - 12x^{-4} = 0$
$x^{-4}(2tx -12) = 0$
$2tx -12 = 0$
$x = \frac{6}{t}$

$f_{t}'''(x) = -6tx^{-4} +48x^{-5}$
$f_{t}'''\left( \frac{6}{t} \right) = -6t\left( \frac{6}{t} \right)^{-4} +48\left( \frac{6}{t} \right)^{-5}$
$= -\frac{6t}{x^4} + \frac{48}{x^5} = \frac{-6tx +48}{x^5}$
$= \frac{-6t \frac{6}{t} +48}{\left( \frac{6}{t} \right)^5} = \frac{12}{\left( \frac{6}{t} \right)^5} \neq 0 \implies W\left( \frac{6}{t} | f_{t}\left( \frac{6}{t} \right) \right)$

$f_{t}\left( \frac{6}{t} \right) = t\cdot \frac{t}{6} -2\cdot \frac{t^2}{36}$
$f_{t}\left( \frac{6}{t} \right) = \frac{t^2}{6} - \frac{t^2}{18}$
$f_{t}\left( \frac{6}{t} \right) = \frac{3t^2}{18} -\frac{t^2}{18} = \frac{t^2}{9}$

$y = \frac{\left( \frac{6}{x} \right)^2}{9} = \frac{36}{9x^2} = \frac{4}{x^2}$
$W(x) = \frac{4}{x^2}$
