
1. Produktregel
	$f(x) = u(x) * v(x)$
	$f'(x) = u'(x) * v(x) + u(x) * v'(x)$
	kurz: $f'(x) = u'v + uv'$

	Bsp.
	$f(x) = x^2*e^x$
	$f'(x) = 2x*e^x + x^2*e^x = e^x*(2x+x^2)$
	$f''(x) = e^x*(2x+x^2) + e^x*(2+2x) = e^x(x^2+4x+2)$
	$f'''(x) = e^x*(x^2+4x+2) + e^x*(2x+4) = e^x*(x^2+6x+6)$

	$f(x) = x^2*\sin x$
	$f'(x) = 2x*\sin x + x^2*\cos x$
	$f''(x) = 2*\sin x+2x*\cos x + 2x*\cos x+x^2*(-\sin x)$
	$= \sin x*(2-x^2) + 4x*\cos x$

	$f(x) = (2x -3) * (3x^2 -4)$
	$f'(x) = 2* (3x^2 -4) + (2x -3) *6x$
	$= 6x^2 -8 +12x^2 -18x$
	$= 18x^2 -18x -8$
	
	other:
	$f(x) = 6x^3 -9x^2 -8x +12$
	$f'(x) = 18x^2 -18x -8$

