
$f(x) = u(v(x))$
$f'(x) = v'(x) \cdot u'(v(x))$

> [!tip] innere Ableitung mal äußere Ableitung

#### Beispiel
$f(x) = \sqrt{x^2 +9} = (x^2 +9)^{\frac12}$
$f'(x) = 2x *\frac12(x^2 +9)^{-\frac12} = x *(x^2 +9)^{-\frac12} = \frac{x}{\sqrt{x^2 +9}}$

#### Beispiel
$f(x) = (3x+7)^8$
$f(x) = 3* 8(3x+7)^7 = 24(3x+7)^{7}$

#### Beispiel
$f(x) = e^{3x-4}$
$f'(x) = 3\cdot e^{3x -4}$

#### Beispiel
$f(x) = \frac{1}{2x -4} = (2x -4)^{-1}$
$f'(x) = 2 *-(2x-4)^{-2} = \frac{-2}{(2x-4)^2}$


> [!important] Spezial Fall: Reziprokenregel
> $f(x) = \frac{1}{v(x)}$
> $f'(x) = \frac{-v'(x)}{(v(x))^2}$

#### Beispiel
$f(x) = (2x +1) *\sin(3x)$
$f'(x) = 2 *\sin(3x) + (2x +1) *3\cos(3x)$

#### Beispiel
$f(x) = \frac{x +2}{x -4} = (x+2)*(x-4)^{-1}$

$f'(x) = 1*(x-4)^{-1} + (x+2)*-(x-4)^{-2}$
$f'(x) = \frac{1}{x-4} - \frac{x+2}{(x -4)^2} = \frac{x-4 - x-2}{(x-4)^2} = \frac{-6}{(x-4)^2}$

##### alternative
$f'(x) = \frac{x-4 -x+2}{(x-4)^2} = \frac{-6}{(x-4)^2}$

#### Beispiel
$f(x) = \frac{3x}{2x-4} = 3x*(2x-4)^{-1}$
$f'(x) = 3*(2x-4)^{-1} + 3x*2*(-1)*(2x-4)^{-2}$
$f'(x) = \frac{3}{2x-4} - \frac{6x}{2x-4}^2 = \frac{3*(2x -4) -6x}{(2x-4)^2} = \frac{-12}{(2x-4)^2}$

##### alternative
$f'(x) = \frac{3*(2x-4) - 3x *2}{(2x-4)^2} = \frac{-12}{(2x -4)^2}$

#### Beispiel
$f(x) = \frac{2x -4}{3x} = \frac{2x}{3x} -\frac{4}{3x} = \frac32 -\frac43x^{-1}$
$f'(x) = \frac43x^{-2}$
