
> [!IMPORTANT] handschriftlich nicht mehr im Lehrplan

$f(x) = \frac{u(x)}{v(x)}$
$f'(x) = \frac{u'(x) *v(x) -u(x) *v'(x)}{(v(x))^2}$
kurz: $(\frac uv)' = \frac{u'v - uv'}{v^2}$

#### Beispiel 3a
$f(x) = \frac{2e^x}{x}$
$f'(x) = \frac{2e^x *x -2e^x *1}{x^2} = \frac{2e^x(x-1)}{x^2}$

#### Beispiel 3b
$f(x) = \frac{5\cos x}{x^2}$
$f'(x) = \frac{-5\sin x *x^2 -5\cos x * 2x}{x^4} = \frac{-5x(x *\sin x + 2\cos x)}{x^4} = \frac{-5(x *\sin x +2\cos x)}{x^3}$

#### Beispiel 3c
$f(x) = \frac{e^x}{x^{-3}} = e^x *x^3$
$f'(x) = \frac{e^x *x^{-3} -e^x*(-3x^{-4})}{x^{-6}} = e^x *x^3 + e^x *3x^2$


