### 1. Konstantenregel
- $f(x) = a$
- $f(x) = 0$

z.B.
- $f(x) = 3$
- $f'(x) = 0$

### 2. Potenzregel
- $f(x) = x^n$
- $f'(x) = n*x^{n-1}$

z.B.
- $f(x) = x^3$
- $f'(x) = n*x^{3-1}$
### 3. Faktorregel
- $f(x) = a*u(x)$
- $f'(x) = a*u'(x)$

z.B.
- $f(x) = 4x^3$
- $f'(x) = 4*3x^2 = 12x^2$

### 4. Summenregel
- $f(x) = u(x) \pm v(x)$
- $f'(x) = u'(x) \pm v'(x)$

z.B.
- $f(x) = 4x^3-8x+1$
- $f'(x) = 4*3x^2 - 8*x^0+0 = 12x^2-8$

#### Beispiele
- $f(x) = 6x^4-8x^3+\frac{3}{4}x^2-\frac{7}{4}x+2$
- $f'(x) = 24x^3 - 24x^2 + \frac{3}{2}x - \frac{7}{4}$

- $f(x) = \frac{4}{x^2} - \frac{2}{x^4} = 4x^{-2}-2x^{-4}$
- $f'(x) = -8x^{-3} + 8x^{-5}$

- $f(x) = 3*\sqrt{x} = 3*x^{\frac{1}{2}}$
- $f'(x) = \frac{3}{2}x^{-\frac{1}{2}} = \frac{3}{2\sqrt{x}}$
