### Nr.2
#### a)
$f'(x) = 5*5x^4 = 25x^{4}$

#### b)
$f'(x) = 12*-3x^{-4} = -36x^{-4}$

#### c)
$f'(x) = 2x^{-\frac{1}{2}} = \frac{2}{\sqrt{x}}$

#### d)
$f'(x) = -\frac233x^2 = -2x^2$

#### e)
$f'(x) = -6x^{-2} = -\frac{6}{x^2}$

#### f)
$f(x) = -\frac35x^{-10}$
$f'(x) = $
$6x^{-11}$
???

#### g)
$f(x) = 10^{-2}*-\frac12x^{-\frac32} = \frac{\frac{-1}{200}}{\sqrt{x}^{3}}$
???

#### h)
$f(x) = \frac122^{-\frac32}*3x^2 = \frac{\frac{3x^2}{2}}{\sqrt{2}^{3}}$
???

### Nr.3
#### a)
$f'(x) = 4x^3+8x^7$

#### b)
$f'(x) = 12x^{11}+-3x^{-2} = 12x^{11}-\frac{3}{x^4}$

#### c)
$f'(x) = -1x^{-2}+4x^3 = 4x^{3}-\frac{1}{x^2}$

#### d)
$f'(x) = -\frac12x^{-\frac32} + 1(x^2)^{-1} = \frac{-\frac{1}{2}}{\sqrt{x}^{3}}+\frac{1}{x^2}$

#### e)
$f'(x) = -1x^{-2} + x = -\frac{1}{x^2} + x$

#### f)
$f'(x) = -10^{-2}*-1*x^{-2}+1 = \frac{\frac{1}{x^2}}{100}+1$
???

#### g)
$f'(x) = -\frac12x^{-\frac32} + 1 = \frac{-\frac{1}{2}}{\sqrt{x}^{3}}+1$
???

#### h)
$f'(x) = 6x$

### Nr. 4
#### a)
$f'(x) = -3*4^\frac12 *8*x^7+10*x^3-2*x^{-1}+4$
???
$f'(x) = -g*x^7+10x^3-2$
#### b)
$f(x) = \frac29x^3+\frac58x^2+0.4x-1.6$
$= 2*9^{-1}x^3 + 5*8^{-1}x^2 + 0.4x - 1.6$
$f'(x) = 2*9^{-1} * 3*x^2 + 5*8^{-1} * 2*x + 0.4 * x^{-1} - 1.6 = \frac{0.4}{x}+0.\overline{6}x^2+1.25x-1.6$
$f'(x) = 2*-1*9^{-2}*3x^2 + 5*-1*8^{-2}*2x + 0.4x - 1.6$
$= -2*9^{-2}*3x^2 + -5*8^{-2}*2x + 0.4x - 1.6$
$= $
???
#### c)
$f'(x) = 3 * 1*x^{-1} + -6*x^{-2} - 5 + 6x^5 = \frac{3}{x}+6x^{5}+\frac{-6}{x^2}-5$
???

#### d)
$f'(x) = -2x^{-\frac12} * x - 20^{-1} * -3x^{-4} - (100x^{9})^{-1} = \frac{\frac{-1}{100}}{x^{9}}-2\sqrt{x}+\frac{\frac{3}{20}}{x^{4}}$
???

#### e)
$f(x) = \frac1{2x} + \sqrt{4x} - x + 1$
$= \frac12x^{-1}+2*x^{\frac12}-x+1$
$f'(x) = -\frac12x^{-2} + x^{-\frac12} - 1$
$= \frac1{\sqrt{x}} - \frac1{2x^2} - 1$

#### f)
$f'(x) = \frac1220^{-\frac12} * x + -(20x)^{-2} + 20x$
???
