## Aufgabe 2
### a)
$f'(x) = 2e^x + 2xe^x = e^x(2 +2x)$

### b)
$f'(x) = 2xe^x + (x^2 + 2)e^x = e^x(2x +x^2+2)$

### c)
$f'(x) = \sqrt{x} + x *\frac12x^{-\frac12} = \frac32x^{\frac12}$

### d)
$f(x) = x^2 * \sqrt{x}$
$f'(x) = 2x *\sqrt x + x^2 *\frac12x^{-\frac12} = \frac52x^{\frac32}$

### e)
$f'(x) = \sin x + x *\cos x$

### f)
$f'(t) = (\cos{t})^2 + \sin t *(-\sin t) = \cos^2t -\sin^2t$

### g)
$f'(x) = -12x^{-4} *e^x + 4x^{-3} *e^x$

### h)
$f(t) = 3t^7 +2t^6 +18t^2 +12t$
$f'(x) = 27t^6 +12t^5 +36t +12$

## Aufgabe 3
### a)
$f(x) = 2e^x *x^{-1}$
$f'(x) = 2e^x *x^{-1} + 2e^x *(-x^{-2}) = 2e^x(x^{-1} -x^{-2})$

### b)
$f(x) = 5\cos x *x^{-2}$
$f'(x) = -5\sin x *x^{-2} + 5\cos x *(-2x^{-3})$

### c)
$f(x) = e^x *x^3$
$f'(x) = e^x *x^3 + e^x *3x^2$

### d)
$f(x) = (x-1) *e^x$
$f'(x) = e^x + (x-1) *e^x$

