## Aufgabe 4
$f(x) = x^2 *e^x$
$f'(x) = 2x *e^x$
$m_0 = f'(0) = 0$
$0 = f'(x)$
$0 = 2x *e^x$ $|:2$
$0 = x *e^x$
$x = 0$
$P(0|0)$
## Aufgabe 5
$f(x) = \frac1x +2x$
$g: y = -\frac23x +\frac53$

$f'(x) = -x^{-2} +2$

$\frac32 = -x^{-2} +2$ $|-\frac32$
$0 = -x^{-2} +\frac12$ $|*-1$
$0 = x^{-2} -\frac12$

## Aufgabe 6
$f(x) = \frac16x^3 -\frac53x^2 +\frac23x$
$g(x) = \frac16x^2 +\frac23x$

$f'(x) = \frac36x^2 -\frac{10}3x +\frac23$
$g'(x) = \frac26x +\frac23$
### a)
$f(x) = g(x)$
$\frac16x^3 -\frac53x^2 +\frac23x = \frac16x^2 +\frac23x$ $|-\frac23x$
$\frac16x^3 -\frac53x^2 = \frac16x^2$ $|*\frac61$
$x^3 -10x^2 = x^2$ $|-x^2$
$0 = x^{3} -11x^2$ $|+11x^2$
$$ x^3 = 11x^2 \implies x = 11$$
$x_1 = 0$ (Regel vom Null-Produkt)
$x_2 = 11$

$P_1(0|0)$
$P_2(11|\frac{165}6)$

$f'(0) = \frac23$
$g'(0) = \frac23$
$f'(0) = g'(0) \implies$ Ber√ºhrungspunkt $B(0|0)$

$f'(11) = \frac{49}{2}$
$g'(11) = \frac{13}{3}$
$f'(11) \neq g'(11) \implies$ Schnittpunkt $S(11|\frac{165}6)$

### b)
$y = \frac{165}6$

$\frac{165}6 = \frac{539}2 +n$ $|-\frac{539}2$
$n = 297$
$t_f(x) = \frac{49}2x +297$

$\frac{165}6 = \frac{143}3 +n$ $|-\frac{143}3$
$n = -\frac{121}{6}$
$t_g(x) = \frac{13}3x -\frac{121}{6}$

