
> [!NOTE] Das Morgansche Gesetzt 
> $\overline{e_1 \land e_2} = \overline{e_1} \lor \overline{e_2}$

$a_1 = e_1 \land e_2$
$a_2 = e_1 \land \overline{e_2}$
$a_3 = \overline{e_1} \land e_2$
$a_4 = \overline{e_1 \lor e_2}$
$a_5 = \overline{e_1 \land e_2}$
$a_6 = \overline{e_1} \lor e_2$
$a_7 = e_1 \lor \overline{e_2}$
$a_8 = e_1 \lor e_2$
$a_9 = \overline{e_1}$
$a_{10} = \overline{e_2}$
$a_{11} = (\overline{e_1} \land \overline{e_2}) \lor (e_1 \land e_2)$
$a_{12} = e_1$
$a_{13} = e_2$
$a_{14} = (\overline{e_1} \lor \overline{e_2}) \lor (e_1 \land e_2)$
$a_{14} = (e_{1} \lor e_{2}) \land (\overline{e_{1}} \lor \overline{e_{2}})$
$a_{15} = 0$
$a_{16} = 1$
